Minor improvements for TreeSync

fstar/new/TreeSync.fst
@@ -23,22 +23,22 @@ let fold f x a = foldi f x a (length x)
 type principal_t = string
 
 type credential_t : eqtype = {
-  name: principal_t;
-  sid: nat;
-  version: nat;
-  identity_key: verif_key_t;
-  issuer: principal_t;
-  signature: bytes_t;
+  cred_name: principal_t;
+  cred_sid: nat;
+  cred_version: nat;
+  cred_identity_key: verif_key_t;
+  cred_issuer: principal_t;
+  cred_signature: bytes_t;
 }
 
 
-let name c = c.name
-let identity_key c = c.identity_key
+let name c = c.cred_name
+let identity_key c = c.cred_identity_key
 assume val validate_: credential_t -> bool
 let valid_credential_p c = validate_ c
 
 (* Secrets associated to a leaf *)
-type leaf_secrets_t : eqtype = {
+type leaf_secrets_t: eqtype = {
   identity_sig_key: sign_key_t;
 }
 
@@ -50,13 +50,13 @@ type node_package_t = {
 }
 
 type tree_t (lev:nat) =
- | Leaf: actor:credential_t{lev=0} -> mi:option leaf_package_t -> tree_t lev
- | Node: actor:credential_t{lev>0} -> kp:option node_package_t ->
+ | Leaf: actor:credential_t{lev=0} -> olp:option leaf_package_t -> tree_t lev
+ | Node: actor:credential_t{lev>0} -> onp:option node_package_t ->
          left:tree_t (lev - 1) -> right:tree_t (lev - 1) -> tree_t lev
 
 type path_t (lev:nat) =
- | PLeaf: mi:option leaf_package_t{lev=0} -> path_t lev
- | PNode: kp:option node_package_t{lev>0} ->
+ | PLeaf: olp:option leaf_package_t{lev=0} -> path_t lev
+ | PNode: onp:option node_package_t{lev>0} ->
 	       next:path_t (lev-1) -> path_t lev
 
 type state_t: eqtype = {
@@ -73,7 +73,7 @@ let group_id g = g.st_group_id
 let max_size g = pow2 g.st_levels
 let epoch g = g.st_epoch
 
-let rec membership_tree (l:nat) (t:tree_t l) : member_array_t (pow2 l) =
+let rec membership_tree (l:nat) (t:tree_t l): member_array_t (pow2 l) =
   match t with
   | Leaf _ mi -> singleton mi
   | Node _ _ left right -> append (membership_tree (l-1) left)
@@ -102,8 +102,7 @@ val create_tree: l:nat -> c:credential_t ->
 		 t:tree_t l{membership_tree l t == init}
 
 (* Create a new tree from a member array *)
-let rec create_tree (l:nat) (c:credential_t)
-		    (init:member_array_t (pow2 l)) =
+let rec create_tree (l:nat) (c:credential_t) (init:member_array_t (pow2 l)) =
   if l = 0 then Leaf c init.[0]
   else let init_l,init_r = split init (pow2 (l-1)) in
     let left = create_tree (l-1) c init_l in
@@ -112,7 +111,7 @@ let rec create_tree (l:nat) (c:credential_t)
 
 (* Auxiliary tree functions *)
 let child_index (l:pos) (i:index_n l) : index_n (l-1) & direction_t =
-  if i < pow2 (l - 1) then (i,Left) else (i-pow2 (l-1),Right)
+  if i < pow2 (l - 1) then (i, Left) else (i-pow2 (l-1), Right)
 
 let order_subtrees dir (l,r) = if dir = Left then (l,r) else (r,l)
 
@@ -121,86 +120,88 @@ let rec apply_path (l:nat) (i:nat{i<pow2 l}) (a:credential_t)
                    (t:tree_t l) (p:path_t l) : tree_t l =
   match t,p with
   | Leaf _ m, PLeaf m' -> Leaf a m'
-  | Node _ _ left right, PNode nk next ->
+  | Node _ _ left right, PNode onp next ->
      let (j,dir) = child_index l i in
      if dir = Left
-     then Node a nk (apply_path (l-1) j a left next) right
-     else Node a nk left (apply_path (l-1) j a right next)
+     then Node a onp (apply_path (l-1) j a left next) right
+     else Node a onp left (apply_path (l-1) j a right next)
 
 (* Create a blank path after modifying a leaf *)
-let rec blank_path (l:nat) (i:index_n l) (mi:option leaf_package_t) : path_t l =
-  if l = 0 then PLeaf mi
+let rec blank_path (l:nat) (i:index_n l) (olp:option leaf_package_t) : path_t l =
+  if l = 0 then PLeaf olp
   else let (j,dir) = child_index l i in
-    PNode None (blank_path (l-1) j mi)
+    PNode None (blank_path (l-1) j olp)
 
-let rec blank_path_lemma (l:nat) (i:index_n l) (mi:option leaf_package_t) (a:credential_t) (t:tree_t l) :
-                    Lemma (let t' = apply_path l i a t (blank_path l i mi) in
-                          membership_tree l t' == ((membership_tree l t).[i] <- mi)) =
+let rec blank_path_lemma (l:nat) (i:index_n l) (olp:option leaf_package_t) (a:credential_t) (t:tree_t l) :
+                    Lemma (let t' = apply_path l i a t (blank_path l i olp) in
+                          membership_tree l t' == ((membership_tree l t).[i] <- olp)) =
     match t with
     | Leaf _ _ ->
-	   let t' = apply_path l i a t (blank_path l i mi) in
-	   Seq.lemma_eq_intro (membership_tree l t') ((membership_tree l t).[i] <- mi)
+	   let t' = apply_path l i a t (blank_path l i olp) in
+	   Seq.lemma_eq_intro (membership_tree l t') ((membership_tree l t).[i] <- olp)
     | Node _ _ left right ->
       let (j,dir) = child_index l i in
       let (child,sibling) = order_subtrees dir (left,right) in
-      let p = PNode None (blank_path (l-1) j mi) in
-      blank_path_lemma (l-1) j mi a child;
-      let t' = apply_path l i a t (blank_path l i mi) in
-      Seq.lemma_eq_intro (membership_tree l t') ((membership_tree l t).[i] <- mi)
+      let p = PNode None (blank_path (l-1) j olp) in
+      blank_path_lemma (l-1) j olp a child;
+      let t' = apply_path l i a t (blank_path l i olp) in
+      Seq.lemma_eq_intro (membership_tree l t') ((membership_tree l t).[i] <- olp)
 
-let initial_leaf_package (mi:option leaf_package_t) =
-  match mi with
+let initial_leaf_package (olp:option leaf_package_t) =
+  match olp with
   | None -> True
-  | Some mi -> valid_credential_p mi.leaf_credential /\ mi.leaf_version = 0
+  | Some lp -> valid_credential_p lp.leaf_credential /\ lp.leaf_version = 0
 
 (* Create an update path from a leaf to the root *)
-let rec update_path (l:nat) (t:tree_t l) (i:nat{i<pow2 l}) (mi_i:leaf_package_t) : option (path_t l) =
+let rec update_path (l:nat) (t:tree_t l) (i:nat{i<pow2 l}) (lp_i:leaf_package_t) : option (path_t l) =
   match t with
   | Leaf _ None -> None
-  | Leaf _ (Some mi) -> if name(mi.leaf_credential) = name(mi_i.leaf_credential)
-                       then Some (PLeaf (Some mi_i))
+  | Leaf _ (Some mi) -> if name(mi.leaf_credential) = name(lp_i.leaf_credential)
+                       then Some (PLeaf (Some lp_i))
                        else None
   | Node _ _ left right ->
      let (j,dir) = child_index l i in
      let (child,sibling) = order_subtrees dir (left,right) in
-     match update_path (l-1) child j mi_i with
+     match update_path (l-1) child j lp_i with
        | None -> None
        | Some next ->
          let np = {node_from = dir; node_content = empty_bytes} in // BB. TODO.
          Some (PNode (Some np) next)
 
-let rec update_path_lemma (l:nat) (i:nat{i<pow2 l}) (a:credential_t) (t:tree_t l) (mi_i:leaf_package_t):
-  Lemma (match update_path l t i mi_i with
+let rec update_path_lemma (l:nat) (i:nat{i<pow2 l}) (a:credential_t) (t:tree_t l) (lp_i:leaf_package_t):
+  Lemma (match update_path l t i lp_i with
 		  | None -> True
 		  | Some p ->
 			 (match (membership_tree l t).[i] with
 			 | None -> False
-			 | Some mi_old -> name(mi_old.leaf_credential) == name(mi_i.leaf_credential) /\
+			 | Some mi_old -> name(mi_old.leaf_credential) == name(lp_i.leaf_credential) /\
 					           (let t' = apply_path l i a t p in
-					           membership_tree l t' = ((membership_tree l t).[i] <- Some mi_i)))) =
+					           membership_tree l t' = ((membership_tree l t).[i] <- Some lp_i)))) =
    match t with
    | Leaf _ None -> ()
    | Leaf _ (Some mi) ->
-     if name(mi.leaf_credential) = name(mi_i.leaf_credential)
-     then let p : path_t l = PLeaf (Some mi_i) in
+     if name(mi.leaf_credential) = name(lp_i.leaf_credential)
+     then let p : path_t l = PLeaf (Some lp_i) in
 	  let t' = apply_path l i a t p in
 	  Seq.lemma_eq_intro (membership_tree l t')
-	                     ((membership_tree l t).[i] <- Some mi_i)
+	                     ((membership_tree l t).[i] <- Some lp_i)
      else ()
   | Node _ _ left right ->
      let (j,dir) = child_index l i in
      let (child,sibling) = order_subtrees dir (left,right) in
-     match update_path (l-1) child j mi_i with
+     match update_path (l-1) child j lp_i with
        | None -> ()
        | Some next ->
-         update_path_lemma (l-1) j a child mi_i;
+         update_path_lemma (l-1) j a child lp_i;
          let np = {node_from = dir; node_content = empty_bytes} in // BB. TODO.
          let p = PNode (Some np) next in
-	 let t' = apply_path l i a t p in
-	 Seq.lemma_eq_intro (membership_tree l t')
-		                 ((membership_tree l t).[i] <- Some mi_i)
+	      let t' = apply_path l i a t p in
+	      Seq.lemma_eq_intro (membership_tree l t')
+		                      ((membership_tree l t).[i] <- Some lp_i)
+
 
 assume val hash_state: state_t -> bytes_t
+
 
 (* Create a new group state *)
 let create gid sz init leaf_secret =
@@ -222,7 +223,7 @@ let create gid sz init leaf_secret =
 		   Some ({g0 with st_transcript_hash = h0}))
 
 val leaf_init: oc:option (c:credential_t) ->
-		    om:option leaf_package_t{
+  om:option leaf_package_t{
 		      match oc,om with
 		      | None,None -> True
 		      | Some c,Some m -> m.leaf_credential == c
@@ -244,10 +245,8 @@ val create_lemma: gid:nat -> sz:pos -> init:member_array_t sz
 	     match create gid sz init entropy with
 	     | None -> True
 	     | Some g ->
-		    group_id g == gid /\  max_size g == sz /\
-		    epoch g == 0      /\
+		    group_id g == gid /\  max_size g == sz /\ epoch g == 0 /\
 		    leaf_updated sz 0 init (membership g))
-
 
 let create_lemma gid sz init leaf_secret =
   match init.[0], log2 sz with
@@ -255,13 +254,13 @@ let create_lemma gid sz init leaf_secret =
   | _,None -> ()
   | Some c,Some l ->
     let t = create_tree l c.leaf_credential init in
-    let mi' = {leaf_credential = c.leaf_credential; leaf_version = 1} in
-    (match update_path l t 0 mi' with
+    let lp' = {leaf_credential = c.leaf_credential; leaf_version = 1} in
+    (match update_path l t 0 lp' with
     | None -> ()
-    | Some p -> (update_path_lemma l 0 c.leaf_credential t mi';
+    | Some p -> (update_path_lemma l 0 c.leaf_credential t lp';
 		   let t' = apply_path l 0 c.leaf_credential t p in
 		   assert (membership_tree l t == init);
-		   assert (membership_tree l t' == ((membership_tree  l t).[0] <- Some mi'));
+		   assert (membership_tree l t' == ((membership_tree  l t).[0] <- Some lp'));
 		   assert (leaf_updated sz 0 (membership_tree l t) (membership_tree l t'))))
 
 
@@ -271,6 +270,7 @@ type operation_t : eqtype= {
   op_actor: credential_t;
   op_path: path_t op_level & path_t op_level
 }
+
 
 assume val hash_op: bytes_t -> operation_t -> bytes_t
 
@@ -284,8 +284,6 @@ let apply g o =
        Some ({g with st_epoch = g.st_epoch + 1; st_tree = t';
   	     st_transcript_hash = hash_op g.st_transcript_hash o})
 
-
-let opt f x = match x with | None -> None | Some x -> Some (f x)
 let update_leaf_package (lp:leaf_package_t) (nc:credential_t) = {
   lp with
   leaf_version = lp.leaf_version + 1;
@@ -293,15 +291,15 @@ let update_leaf_package (lp:leaf_package_t) (nc:credential_t) = {
 }
 
 (* Create an operation that modifies the group state *)
-let modify g actor i oleaf_package =
+let modify g actor i olp =
   match (membership g).[actor] with
   | None -> None
   | Some mi_a_old ->
-    match oleaf_package with
+    match olp with
     | None -> None
     | Some lp ->
       let mi_a = update_leaf_package mi_a_old lp.leaf_credential in
-      let bp = blank_path g.st_levels i oleaf_package in
+      let bp = blank_path g.st_levels i olp in
       let nt = apply_path g.st_levels i mi_a.leaf_credential g.st_tree bp in
       match update_path g.st_levels nt i mi_a with
       | None -> None
